Removed restriction that goal must be a conjunction. Added step to turn goal into an auxiliary action + dummy goal. Proved degoal domain wf. Added DNF logic.

Formula_Normalization.thy
@@ -1,6 +1,6 @@
 theory Formula_Normalization
 imports "AI_Planning_Languages_Semantics.PDDL_STRIPS_Semantics"
-    Type_Normalization Utils AbLa_alts
+    Type_Normalization Utils AbLa_alts DNF
 begin
 
 
@@ -12,8 +12,44 @@ locale type_normed_problem = wf_ast_problem +
 
 context ast_domain begin
 
+(* G for goal *)
+definition "dummy_pred \<equiv> Pred (safe_prefix pred_names @ ''G'')"
+definition "dummy_pred_decl \<equiv> PredDecl dummy_pred []"
+
+fun set_pre :: "ast_action_schema \<Rightarrow> term atom formula \<Rightarrow> ast_action_schema" where
+  "set_pre (Action_Schema n params _ eff) pre = Action_Schema n params pre eff"
+
+fun split_ac :: "ast_action_schema \<Rightarrow> ast_action_schema list" where
+  "split_ac ac =
+    map (set_pre ac) (dnf_list (ac_pre ac))"
+
+definition "split_acs \<equiv> concat (map split_ac (actions D))"
+
+fun dummy_ac where "dummy_ac (c, s) =
+  Action_Schema s [] c (Effect [Atom (predAtm dummy_pred [])] [])"
+
+abbreviation "ac_names \<equiv> map ac_name (actions D)"
+
+definition "dummy_ac_names clauses \<equiv>
+  (map ((@) (safe_prefix ac_names)) (distinct_strings (length clauses)))"
+
+definition "dummy_acs g \<equiv>
+  map dummy_ac (zip (dnf_list g) (dummy_ac_names (dnf_list g)))"
+
+end
+
+context ast_problem begin
+
+definition "fmla_normed_dom \<equiv>
+  Domain
+    (types D)
+    (dummy_pred_decl # predicates D)
+    (consts D)
+    split_acs"
 
 
+definition "fmla_normed_prob \<equiv>
+  Problem fmla_normed_dom (objects P) (init P) (goal P)" (* TODO dummy goal *)
 
 end
 
