String_Shenanigans.thy
@@ -1,5 +1,5 @@
 theory String_Shenanigans
-imports Main
+imports Main "Show.Show_Instances"
 begin
 
 fun max_length :: "'a list list \<Rightarrow> nat" where
@@ -15,16 +15,66 @@ definition safe_prefix :: "string list \<Rightarrow> string" where
 lemma safe_prefix_correct: "safe_prefix xs @ x \<notin> set xs"
   using max_length_correct safe_prefix_def by force
 
+lemma dist_prefix: "distinct xs \<Longrightarrow> distinct (map ((@) (safe_prefix ys)) xs)"
+  by (simp add: distinct_conv_nth)
+
+
+(* padding *)
+
+definition pad :: "nat \<Rightarrow> string \<Rightarrow> string" where
+  "pad n s \<equiv> s @ replicate (n - length s) (CHR ''_'')"
+
+lemma pad_length:
+  "n \<ge> length s \<Longrightarrow> length (pad n s) = n"
+  "length (pad n s) \<ge> n"
+  "length (pad n s) \<ge> length s"
+  unfolding pad_def by simp_all
+
+definition make_unique :: "string list \<Rightarrow> string \<Rightarrow> string" where
+  "make_unique ss s \<equiv> pad (max_length ss + 1) s"
+
+lemma made_unique: "make_unique ss x \<notin> set ss"
+proof -
+  have "max_length ss + 1 \<le> length (make_unique ss x)"
+    using make_unique_def pad_length(2) by simp
+  hence "\<forall>s \<in> set ss. length s < length (make_unique ss x)"
+    using max_length_correct by fastforce
+  thus ?thesis by auto
+qed
+
+
+definition pad_strings :: "string list \<Rightarrow> string list" where
+  "pad_strings ss \<equiv> map (pad (max_length ss + 1)) ss"
+
+lemma
+  assumes "distinct xs"
+    "\<forall>y \<in> set ys. length y = n"
+  shows "distinct (map2 (@) ys xs)"
+  using assms oops
+
+lemma show_nat_inj: fixes a :: nat and b :: nat assumes "a \<noteq> b" shows "show a \<noteq> show b"
+  using assms sorry
+
+fun nat_upto :: "nat \<Rightarrow> nat list" where
+  "nat_upto 0 = [0]" |
+  "nat_upto (Suc n) = Suc n # nat_upto n"
+
+definition "distinct_strings n \<equiv> map show (case n of 0 \<Rightarrow> [] | Suc m \<Rightarrow> nat_upto m)"
+
+
+lemma dist_str_props:
+  "length (distinct_strings n) = n"
+  "distinct (distinct_strings n)"
+  sorry
+
+
 definition distinctize :: "string list \<Rightarrow> string list \<Rightarrow> string list" where
   "distinctize blocked new \<equiv>
     map (append (safe_prefix blocked)) new"
 
-lemma distinctize_correct:
+(*lemma distinctize_correct:
   "disjnt (set blocked) (set (distinctize blocked new))"
-  by (metis (no_types, opaque_lifting) disjnt_iff distinctize_def ex_map_conv safe_prefix_correct)
-
-lemma dist_prefix: "distinct xs \<Longrightarrow> distinct (map ((@) (safe_prefix ys)) xs)"
-  by (simp add: distinct_conv_nth)
+  by (metis (no_types, opaque_lifting) disjnt_iff distinctize_def ex_map_conv safe_prefix_correct)*)
 
 
 end
