DNF.thy
@@ -1,0 +1,106 @@
+theory DNF
+imports
+    "Propositional_Proof_Systems.CNF"
+    "Propositional_Proof_Systems.CNF_Formulas"
+    "Propositional_Proof_Systems.CNF_Sema"
+    "Propositional_Proof_Systems.CNF_Formulas_Sema"
+    "Verified_SAT_Based_AI_Planning.CNF_Supplement"
+    "Verified_SAT_Based_AI_Planning.CNF_Semantics_Supplement"
+    Utils
+begin
+
+subsection \<open>DNF construction\<close>
+
+fun is_conj where
+  "is_conj (F \<^bold>\<and> G) \<longleftrightarrow> is_lit_plus F \<and> is_conj G" |
+  "is_conj H \<longleftrightarrow> is_lit_plus H"
+
+fun is_dnf where
+  "is_dnf (F \<^bold>\<or> G) \<longleftrightarrow> is_dnf F \<and> is_dnf G" |
+  "is_dnf H \<longleftrightarrow> is_conj H"
+
+lemma lit_neg_lit:
+  assumes "is_lit_plus F"
+  shows "is_lit_plus (nnf (\<^bold>\<not> F))"
+  using assms apply (induction F) apply simp_all
+  using is_nnf_NotD by force
+
+lemma disj_neg_conj:
+  assumes "is_disj F"
+  shows "is_conj (nnf (\<^bold>\<not> F))"
+using assms proof (induction F)
+  case Not then show ?case using is_nnf_NotD by fastforce
+qed (auto simp add: lit_neg_lit)
+
+lemma cnf_to_dnf:
+  assumes "is_cnf F"
+  shows "is_dnf (nnf (\<^bold>\<not> F))"
+using assms proof (induction F)
+  case Not
+  then show ?case using is_nnf_NotD by fastforce
+next
+  case Or
+  thus ?case using lit_neg_lit disj_neg_conj by auto
+qed simp_all
+
+definition "dnf F \<equiv> nnf (\<^bold>\<not> (cnf_form_of (nnf F)))"
+
+lemma is_dnf_dnf: "is_dnf (dnf F)" unfolding dnf_def
+  using is_nnf_nnf cnf_form_of_is cnf_to_dnf by blast
+
+subsection \<open>Straight to transformation\<close>
+
+primrec neg_of_lit where
+"neg_of_lit (Pos k) = \<^bold>\<not>(Atom k)" |
+"neg_of_lit (Neg k) = Atom k"
+
+lemma neg_lit_semantics:
+  "A \<Turnstile> form_of_lit l \<longleftrightarrow> \<not> A \<Turnstile> neg_of_lit l"
+  by (cases l) simp_all
+
+definition "neg_conj_of_clause c \<equiv> \<^bold>\<And>[neg_of_lit l. l \<leftarrow> c]"
+
+lemma neg_conj_semantics: "A \<Turnstile> neg_conj_of_clause c \<longleftrightarrow> \<not> A \<Turnstile> disj_of_clause c"
+proof -
+  have "A \<Turnstile> disj_of_clause c \<longleftrightarrow> (\<exists>l \<in> set (map form_of_lit c). A \<Turnstile> l)"
+    using disj_of_clause_def BigOr_semantics by metis
+  also have "... \<longleftrightarrow> (\<exists>l \<in> set c. A \<Turnstile> form_of_lit l)"
+    by simp
+  also have "... \<longleftrightarrow> (\<exists>l \<in> set c. \<not>A \<Turnstile> neg_of_lit l)"
+    using neg_lit_semantics by auto
+  also have "... \<longleftrightarrow> \<not>(\<forall>l \<in> set c. A \<Turnstile> neg_of_lit l)"
+    using neg_lit_semantics by auto
+  also have "... \<longleftrightarrow> \<not>(\<forall>l \<in> set (map neg_of_lit c). A \<Turnstile> l)"
+    by simp
+  also have "... \<longleftrightarrow> \<not> A \<Turnstile> neg_conj_of_clause c"
+    using neg_conj_of_clause_def BigAnd_semantics by metis
+  finally show ?thesis by simp
+qed
+
+definition dnf_list :: "'a formula \<Rightarrow> 'a formula list" where
+  "dnf_list F \<equiv> map (neg_conj_of_clause) (cnf_lists (nnf (\<^bold>\<not>F)))"
+
+lemma dnf_list_semantics:
+  fixes F :: "'a formula"
+  shows "(A \<Turnstile> F) \<longleftrightarrow> (\<exists>c \<in> set (dnf_list F). A \<Turnstile> c)"
+proof -
+  define nF where "nF \<equiv> nnf (\<^bold>\<not>F)"
+  have "A \<Turnstile> F \<longleftrightarrow> \<not> A \<Turnstile> nF"
+    using nnf_semantics nF_def by force
+  also have "... \<longleftrightarrow> \<not> A \<Turnstile> (form_of_cnf \<circ> cnf_lists) nF"
+    using nF_def is_nnf_nnf cnf_form_semantics cnf_form_of_def by metis
+  also have "... \<longleftrightarrow> \<not> A \<Turnstile> \<^bold>\<And>(map disj_of_clause (cnf_lists nF))"
+    unfolding form_of_cnf_def by simp
+  also have "... \<longleftrightarrow> \<not>(\<forall>c \<in> set (cnf_lists nF). A \<Turnstile> disj_of_clause c)"
+    by simp
+  also have "... \<longleftrightarrow> (\<exists>c \<in> set (cnf_lists nF). A \<Turnstile> neg_conj_of_clause c)"
+    using neg_conj_semantics by auto
+  also have "... \<longleftrightarrow> (\<exists>c \<in> set (map neg_conj_of_clause (cnf_lists nF)). A \<Turnstile> c)"
+    using nF_def by simp
+  finally show ?thesis using nF_def dnf_list_def by metis
+qed
+
+
+
+
+end
