Goal_Normalization.thy
@@ -1,0 +1,262 @@
+theory Goal_Normalization
+imports "AI_Planning_Languages_Semantics.PDDL_STRIPS_Semantics"
+    Type_Normalization Utils AbLa_alts DNF
+begin
+
+context ast_domain begin
+
+  definition "goal_pred \<equiv> Pred (make_unique pred_names ''Goal'')"
+  definition "goal_pred_decl \<equiv> PredDecl goal_pred []"
+  
+  abbreviation "ac_names \<equiv> map ac_name (actions D)"
+  
+  abbreviation "goal_ac_name \<equiv> make_unique ac_names ''Goal''"
+  
+  abbreviation "goal_effect \<equiv> Effect [Atom (predAtm goal_pred [])] []"
+  
+  definition goal_ac where "goal_ac g =
+    Action_Schema goal_ac_name [] g goal_effect"
+end
+
+definition "obj_to_term obj \<equiv> term.VAR obj"
+
+context ast_problem begin
+
+  definition "term_goal \<equiv> (map_formula\<circ>map_atom) term.CONST (goal P)"
+  
+  definition "degoal_dom \<equiv>
+    Domain
+      (types D)
+      (goal_pred_decl # predicates D)
+      (objects P @ consts D)
+      (goal_ac term_goal # actions D)"
+  
+  definition "degoal_prob \<equiv>
+    Problem
+      degoal_dom
+      []
+      (init P)
+      (Atom (predAtm goal_pred []))"
+
+end
+
+abbreviation (in ast_problem) (input) "D3 \<equiv> degoal_dom"
+abbreviation (in ast_problem) (input) "P3 \<equiv> degoal_prob"
+
+locale ast_problem3 = ast_problem
+sublocale ast_problem3 \<subseteq> d3: ast_domain D3 .
+sublocale ast_problem3 \<subseteq> p3: ast_problem P3 .
+
+locale wf_ast_problem3 = wf_ast_problem
+sublocale wf_ast_problem3 \<subseteq> d3: ast_domain D3 .
+sublocale wf_ast_problem3 \<subseteq> p3: ast_problem P3 .
+
+subsection \<open> Alternate/simplified definitions\<close>
+context ast_problem begin
+
+lemma degoal_dom_sel:
+  "types D3 = types D"
+  "predicates D3 = goal_pred_decl # predicates D"
+  "consts D3 = objects P @ consts D"
+  "actions D3 = goal_ac term_goal # actions D"
+  using degoal_dom_def by simp_all
+
+lemma degoal_prob_sel:
+  "domain P3 = degoal_dom"
+  "objects P3 = []"
+  "init P3 = init P"
+  "goal P3 = Atom (predAtm goal_pred [])"
+  using degoal_prob_def by simp_all
+end
+
+subsection \<open>Well-Formedness\<close>
+
+context wf_ast_problem3 begin
+
+
+lemma pred_stack: "Pred ` predicate.name ` ps = ps" by force
+
+lemma g_preds_dist: "distinct (map pred (predicates D3))"
+proof -
+  have "make_unique pred_names ''Goal'' \<notin> set pred_names"
+    using made_unique by blast
+  hence "make_unique pred_names ''Goal'' \<notin> predicate.name ` (pred ` set (predicates D))"
+    by auto
+  hence "goal_pred \<notin> pred ` set (predicates D)"
+    unfolding goal_pred_def using pred_stack by blast
+  hence "pred goal_pred_decl \<notin> pred ` set (predicates D)"
+    using goal_pred_decl_def by force
+  thus ?thesis
+    using wf_D(2) degoal_dom_sel(2) by auto
+qed
+
+lemma g_type_wf: "wf_type T \<Longrightarrow> d3.wf_type T"
+  using degoal_dom_sel(1) by (cases T) simp
+
+lemma g_preds_wf: "list_all1 d3.wf_predicate_decl (predicates D3)"
+proof -
+  have "wf_predicate_decl pd \<Longrightarrow> d3.wf_predicate_decl pd" for pd
+    using g_type_wf by (cases pd) simp
+
+  hence "list_all1 d3.wf_predicate_decl (predicates D)"
+    using wf_D(3) degoal_dom_sel(2) by simp
+  moreover have "d3.wf_predicate_decl goal_pred_decl"
+    unfolding goal_pred_decl_def by simp
+
+  ultimately show ?thesis using degoal_dom_sel(2) by simp
+qed
+
+lemma g_acs_dist: "distinct (map ac_name (actions D3))"
+proof -
+  have "goal_ac_name \<notin> set ac_names"
+    using made_unique by blast
+  hence "ac_name (goal_ac term_goal) \<notin> ac_name ` set (actions D)"
+    using ast_domain.goal_ac_def by fastforce
+  thus ?thesis using degoal_dom_sel wf_D(6) by auto
+qed
+
+thm wf_action_schema.simps
+thm wf_action_schema_alt
+
+lemma g_sig:
+  assumes "sig p = Some xs" shows "d3.sig p = Some xs"
+proof -
+  from assms have "PredDecl p xs \<in> set (predicates D3)"
+    using sig_Some degoal_dom_sel by simp
+  thus ?thesis using pred_resolve g_preds_dist degoal_dom_sel d3.sig_def by metis
+qed
+
+lemma g_fmla_wf:
+  assumes "wf_fmla tyt \<phi>" shows "d3.wf_fmla tyt \<phi>"
+  using assms
+proof (induction \<phi>)
+  case (Atom x) thus ?case
+  proof (cases x)
+    case (predAtm p xs)
+    hence a: "wf_pred_atom tyt (p, xs)" using assms Atom by simp
+    then obtain Ts where sig: "sig p = Some Ts"
+      by fastforce
+    with a have "list_all2 (is_of_type tyt) xs Ts" by simp
+    hence "list_all2 (d3.is_of_type tyt) xs Ts"
+      unfolding ast_domain.is_of_type_def ast_domain.of_type_def ast_domain.subtype_rel_def degoal_dom_sel(1)
+      by simp
+    moreover have "d3.sig p = Some Ts" using g_sig sig by simp
+    ultimately have "d3.wf_pred_atom tyt (p, xs)" by simp
+    then show ?thesis using predAtm by simp
+  qed simp
+qed auto
+
+lemma g_constT:
+  "objT = d3.constT"
+  using objT_def degoal_dom_sel d3.constT_def
+  using constT_def map_le_iff_map_add_commute objm_le_objT by auto
+
+lemma g_eff_wf:
+  assumes "wf_effect tyt \<epsilon>" shows "d3.wf_effect tyt \<epsilon>"
+  using assms apply (cases \<epsilon>; simp)
+  using ast_domain.wf_fmla_atom_alt g_fmla_wf by blast
+
+lemma wf_fmla_mono:
+  assumes "tys \<subseteq>\<^sub>m tys'" "wf_fmla tys \<phi>"
+  shows "wf_fmla tys' \<phi>"
+  using assms apply (induction \<phi>)
+  apply (simp add: wf_atom_mono) by simp_all
+
+lemma wf_eff_mono:
+  assumes "tys \<subseteq>\<^sub>m tys'" "wf_effect tys eff"
+  shows "wf_effect tys' eff"
+  using assms apply (cases eff)
+  using wf_fmla_atom_mono by auto
+
+lemma wf_atom_to_term:
+  assumes "wf_atom tyt a"
+  shows "wf_atom (ty_term xd tyt) (map_atom term.CONST a)"
+proof (cases a)
+  case (predAtm p xs)
+  with assms obtain Ts where sig: "sig p = Some Ts" by fastforce
+  from sig have match: "list_all2 (is_of_type tyt) xs Ts" using predAtm assms by simp
+
+  have "list_all2 (is_of_type (ty_term xd tyt)) (map term.CONST xs) Ts"
+    using match
+  proof (induction xs arbitrary: Ts)
+    case (Cons g gs)
+    then obtain t ts where ts: "t # ts = Ts"
+      by (metis list_all2_Cons1)
+    with Cons have 1: "is_of_type tyt g t" "list_all2 (is_of_type tyt) gs ts"
+      by auto
+    hence "list_all2 (is_of_type (ty_term xd tyt)) (map term.CONST gs) ts"
+      "is_of_type (ty_term xd tyt) (term.CONST g) t"
+      using Cons.IH apply simp
+      using 1 by (simp add: ast_domain.is_of_type_def)
+    thus ?case using ts list_all2_Cons1 by auto
+  qed simp
+
+  thus ?thesis using predAtm sig by simp
+next
+  case Eq thus ?thesis using assms by auto
+qed
+
+lemma wf_fmla_to_term:
+  assumes "wf_fmla tyt F"
+  shows "wf_fmla (ty_term xd tyt) ((map_formula \<circ> map_atom) term.CONST F)"
+  using assms by (induction F) (simp_all add: wf_atom_to_term)
+
+lemma g_acs_wf: "(\<forall>a\<in>set (actions D3). d3.wf_action_schema a)"
+proof -
+  have 1: "d3.wf_action_schema ac" if "wf_action_schema ac" for ac
+  proof (cases ac)
+    case (Action_Schema n params pre eff)
+
+    let ?tyt = "ty_term (map_of params) constT"
+    let ?tyt3 = "ty_term (map_of params) d3.constT"
+    have tyts: "?tyt \<subseteq>\<^sub>m ?tyt3"
+      using degoal_dom_sel ast_domain.constT_def g_constT constT_ss_objT
+      by (simp add: ty_term_mono)
+
+    from that have "wf_fmla ?tyt pre \<and> wf_effect ?tyt eff"
+      by (metis Action_Schema ast_domain.wf_action_schema.simps)
+    hence "d3.wf_fmla ?tyt3 pre \<and> d3.wf_effect ?tyt3 eff" using tyts wf_fmla_mono wf_eff_mono
+      using g_eff_wf g_fmla_wf by blast
+    moreover have "distinct (map fst params)" using Action_Schema that by (meson wf_action_schema.simps)    
+    ultimately show ?thesis using Action_Schema ast_domain.wf_action_schema.simps by simp
+  qed
+
+  let ?gac = "goal_ac term_goal"
+  have "d3.wf_action_schema ?gac"
+  proof -
+    have 1: "distinct (map fst (ac_params ?gac))"
+      unfolding goal_ac_def by (cases ?gac) simp
+    let ?tyt = "ty_term Map.empty d3.constT"
+    have 2: "d3.wf_fmla ?tyt term_goal"
+      unfolding term_goal_def
+      using wf_P g_constT wf_fmla_to_term g_fmla_wf by metis
+    have 3: "d3.wf_effect ?tyt goal_effect"
+      (* d_preds_dist not needed, since goal_pred is the first in the list *)
+      using degoal_dom_sel(2) d3.sig_def goal_pred_decl_def by force
+    from 1 2 3 show ?thesis
+      by (simp add: goal_ac_def)
+
+  qed
+  with 1 show ?thesis using wf_D(7) degoal_dom_sel by simp
+qed
+
+lemma degoal_dom_wf: "d3.wf_domain"
+proof -
+  note degoal_dom_sel[simp]
+  have c1: "d3.wf_types" using ast_domain.wf_types_def wf_D by simp
+  note c2 = g_preds_dist
+  note c3 = g_preds_wf
+  have c4: "distinct (map fst (consts D3))" using wf_D wf_P by simp
+  have c5: "\<forall>(n, T) \<in> set (consts D3). d3.wf_type T" using wf_D wf_P g_type_wf by auto
+  note c6 = g_acs_dist
+  note c7 = g_acs_wf
+  from c1 c2 c3 c4 c5 c6 c7 show ?thesis using d3.wf_domain_def by simp
+qed
+
+end
+
+
+sublocale restr_domain2 \<subseteq> d2: wf_ast_domain D2
+  using detype_dom_wf wf_ast_domain.intro by simp
+
+end
